src/parse/type_pp.sig
@@ -4,4 +4,5 @@ sig
  val pp_type : type_grammar.grammar -> Portable.ppstream -> Type.hol_type -> unit
  val pp_type_with_depth :
   type_grammar.grammar -> Portable.ppstream -> int -> Type.hol_type -> unit
+ val pp_num_types : bool ref
 end
